add: implementation of priority queue, not following the contract yet

source/PriorityQueue.dfy
@@ -1,8 +1,9 @@
 include "Queue.dfy"
 
-function method emptyLists<T>(size : nat) : seq<seq<T>>
+function emptyLists<T>(size : nat) : seq<seq<T>>
 	ensures |emptyLists<T>(size)| == size
 	ensures forall i :: 0 <= i < size ==> emptyLists<T>(size)[i] == []
+	ensures flatten(emptyLists<T>(size)) == []
 {
 	if size == 0 then
 		[]
@@ -10,7 +11,7 @@ function method emptyLists<T>(size : nat) : seq<seq<T>>
 		[[]] + emptyLists(size - 1)
 }
 
-function method flatten<T>(sequences : seq<seq<T>>) : seq<T>
+function flatten<T>(sequences : seq<seq<T>>) : seq<T>
 {
 	if sequences == [] then
 		[]
@@ -18,38 +19,64 @@ function method flatten<T>(sequences : seq<seq<T>>) : seq<T>
 		sequences[0] + flatten(sequences[1..])
 }
 
+lemma flattenNonEmptyImpliesSomeElement<T>(sequences : seq<seq<T>>)
+	ensures flatten(sequences) != [] <==> exists i :: 0 <= i < |sequences| && sequences[i] != []
+{
+	if flatten(sequences) == [] {
+		assert forall i :: 0 <= i < |sequences| ==> sequences[i] == [];
+	} else if sequences[0] == [] {
+		flattenNonEmptyImpliesSomeElement(sequences[1..]);
+	} else {
+		assert sequences[0] != [];
+	}
+}
+
+function firstNonEmpty<T>(sequences : seq<seq<T>>) : nat
+	requires flatten<T>(sequences) != []
+	requires |sequences| > 0
+	ensures 0 <= firstNonEmpty(sequences) < |sequences|
+	ensures |sequences[firstNonEmpty(sequences)]| > 0
+	ensures forall k :: 0 <= k < |sequences| && sequences[k] != []
+	==> firstNonEmpty(sequences) <= k
+	decreases |sequences|
+{
+	if sequences[0] != [] then
+		0
+	else
+		1 + firstNonEmpty(sequences[1..])
+}
+
+const maxPriority := 3;
+
 class {:autocontracts} PriorityQueue<T>
 {
-	const maxPriority : nat;
+	// const maxPriority : nat;
 	var queues : array<Queue<T>>;
+	var elements : nat;
 	ghost var sequences : seq<seq<T>>;
 
-	constructor(maxPriority : nat, default : nat -> Queue<T>)
-		ensures this.maxPriority == maxPriority
+	constructor(default : T)
+		// ensures this.maxPriority == maxPriority
 		ensures sequences == emptyLists(maxPriority)
+		ensures flatten(sequences) == []
 		ensures queues.Length == maxPriority
 	{
-		this.maxPriority := maxPriority;
+		// this.maxPriority := maxPriority;
 		new;
-		this.queues := new Queue<T>[maxPriority](default);
+		this.elements := 0;
+		var initializer := new Queue<T>(default);
+		this.queues := new Queue<T>[maxPriority]((_) => initializer);
 		this.sequences := emptyLists(maxPriority);
-	}
+		// this.Repr := {this, queues[0], queues[1], queues[2]};
+	} 
 
 	predicate Valid()
 	{
 		&& |sequences| == maxPriority
 		&& queues.Length == maxPriority
-		&& forall i :: 0 <= i < |sequences| ==> sequences[i] == queues[i].elemSeq	
-	}
-
-	method size() returns (result : nat)
-		ensures result == |flatten(sequences)|
-	{
-		result := 0;
-		forall i | 0 <= i < queues.Length
-		{
-			result := result + queues[i].size();
-		}
+		&& elements == |flatten(sequences)|
+		&& forall i :: 0 <= i < maxPriority ==> queues[i].Valid()
+		&& forall i :: 0 <= i < maxPriority ==> sequences[i] == queues[i].elemSeq	
 	}
 
 	function index(priority : nat) : nat
@@ -65,42 +92,83 @@ class {:autocontracts} PriorityQueue<T>
 	{
 		index + 1
 	}
-		
-	method empty() returns (result : bool)
-		ensures result <==> (|flatten(sequences)| == 0)
+
+	function method size() : nat
+		ensures size() == |flatten(sequences)|
 	{
-		var size := size();
-		result := (size == 0);
+		elements
+	}
+		
+	predicate method empty()
+		ensures empty() <==> (size() == 0)
+	{
+		size() == 0
 	}
 
-	function minPriority() : nat
-		requires |flatten(sequences)| > 0
-		ensures 0 < minPriority() <= maxPriority
-		ensures |sequences[index(minPriority())]| > 0
+	function minPriorityFunc() : nat
+		requires !empty()
+		ensures 0 < minPriorityFunc() <= maxPriority
+		ensures |sequences[index(minPriorityFunc())]| > 0
 		ensures forall k :: 0 <= k < |sequences| && sequences[k] != []
-		==> index(minPriority()) <= k
+		==> index(minPriorityFunc()) <= k
+	{
+		priority(firstNonEmpty(sequences))
+	}
+
+	method minPriority() returns (min : nat)
+		requires !empty()
+		ensures min == minPriorityFunc()
+		ensures 0 < min <= maxPriority
+		ensures |sequences[index(min)]| > 0
+		ensures forall k :: 0 <= k < |sequences| && sequences[k] != []
+		==> index(min) <= k
+	{
+		var i := 0;
+		assert !empty();
+		assert flatten(sequences) != [];
+		assert exists i :: 0 <= i < maxPriority && sequences[i] != [];
+		while i < maxPriority
+			invariant 0 <= i < maxPriority
+			invariant forall j :: 0 <= j < i ==> sequences[j] == []
+			invariant exists j :: i <= j < maxPriority && sequences[j] != []
+		{
+			if (queues[i].size() > 0)
+			{
+				break;
+			}
+			i := i + 1;
+		}
+		min := i;
+	}
 
 	method push(value : T, priority : nat)
 		requires 0 < priority <= maxPriority
 		ensures sequences[index(priority)] == old(sequences[index(priority)]) + [value]
-		// ensures size() == old(size()) + 1
+		ensures size() == old(size()) + 1
 		ensures forall k :: 0 <= k < |sequences| && k != index(priority)
 		==> sequences[k] == old(sequences[k])
+	{
+		queues[index(priority)].push(value);
+		sequences[index(priority)] := sequences[index(priority)] + [value]; 
+	}
 
 	method pop() returns (result : T)
-		requires |flatten(sequences)| > 0
-		ensures result == old(sequences[index(minPriority())][0])
-		ensures sequences[old(index(minPriority()))] == old(sequences[index(minPriority())][1..])
-		// ensures size() == old(size()) - 1
-		ensures forall k :: 0 <= k < |sequences| && k != old(index(minPriority()))
+		requires !empty()
+		ensures result == old(sequences[index(minPriorityFunc())][0])
+		ensures sequences[old(index(minPriorityFunc()))] == old(sequences[index(minPriorityFunc())][1..])
+		ensures size() == old(size()) - 1
+		ensures forall k :: 0 <= k < |sequences| && k != old(index(minPriorityFunc()))
 		==> sequences[k] == old(sequences[k])
+	{
+		var priority := minPriority();
+		result := queues[priority].pop();
+		sequences[priority] := sequences[priority][1..];
+	}
 }
 
 method TestPriorityQueue()
 {
-	var initializer : nat -> Queue<int> := (_) => (new Queue<int>(0));
-	var a := new Queue<int>(0);
-	var q := new PriorityQueue<int>(3, initializer);
+	var q := new PriorityQueue<int>(0);
 	q.push(2, 1);
 	q.push(-3, 3);
 	q.push(5, 2);
